src/Log/Specs.v
@@ -1,6 +1,7 @@
 Require Import Primitives BatchOperations Layer1.
-Require Import Log.Definitions.
-Require Import Datatypes.
+Require Import Log.Definitions Log.LogParameters.
+Require Import Datatypes PeanoNat Omega.
+Import Nat.
 
 Set Nested Proofs Allowed.
 
@@ -61,7 +62,172 @@ Definition commit (addr_l data_l: list value) :=
   else
     Ret false.
 
-*)
+ *)
+
+Lemma log_rep_extract_header_block:
+  forall a hdr log_blocks,
+    log_rep hdr log_blocks a =*=>
+    exists* hdr_block,
+      ((hdr_block_num |-> hdr_block *
+       (hdr_block_num |-> hdr_block --* log_rep hdr log_blocks a)) *
+       [[ decode_header (fst hdr_block) = hdr ]]).
+Proof.
+  unfold log_rep, log_rep_inner; intros.
+  norml.
+  exists hdr_block.
+  apply sep_star_lift_apply'; eauto.
+  setoid_rewrite <- septract_pimpl_r.
+  apply sep_star_comm.
+  apply septract_sep_star_extract.
+  2: eauto.
+  cancel.
+  cancel.
+Qed.
+
+Lemma pred_array_split:
+  forall V (l: list V) n a,
+    a |=> l =*=> a |=> firstn n l * (a+n) |=> skipn n l.
+Proof.
+  induction l; intros.
+  {
+    simpl.
+    rewrite firstn_nil, skipn_nil; simpl; cancel.
+  }
+  {
+    destruct n; simpl.
+    - rewrite add_0_r; cancel.
+    - cancel.
+      rewrite <- add_succ_comm; eauto.
+  }
+Qed.
+
+Lemma pred_array_merge:
+  forall V (l: list V) n a,
+    a |=> firstn n l * (a+n) |=> skipn n l =*=> a |=> l.
+Proof.
+  induction l; intros.
+  {
+    simpl.
+    rewrite firstn_nil, skipn_nil; simpl; cancel.
+  }
+  {
+    destruct n; simpl.
+    - rewrite add_0_r; cancel.
+    - cancel.
+      rewrite <- add_succ_comm; eauto.
+      rewrite <- IHl; cancel.
+  }
+Qed.
+
+Theorem log_write_consecutive_ok :
+  forall vl start log_blocks hdr o d a,
+    let log_index := start - log_start in
+    let new_log_blocks :=
+        firstn log_index log_blocks ++ vl ++
+        skipn (log_index + length vl) log_blocks in  
+    << o, d, a >>
+      (log_rep hdr log_blocks a *
+       [[ start >= log_start + cur_count hdr ]] *
+       [[ start + length vl < log_start + log_length ]])
+      (write_consecutive start vl)
+    << r, ar >>               
+      (log_rep hdr new_log_blocks ar *
+       [[ ar = a ]])%pred
+      (exists* n,
+         let partially_new_log_blocks :=
+             firstn log_index log_blocks ++ firstn n vl ++
+             skipn (log_index + n) log_blocks in
+      log_rep hdr partially_new_log_blocks ar *
+      [[ n <= length vl ]] *
+      [[ ar = a ]])%pred.
+Proof.
+  unfold log_rep; intros.
+  eapply pre_impl.
+  2:
+    eassign
+       (fun (_:oracle) a =>
+          (exists* (log_blockset : list data)  (hdr_block : data),
+             hdr_block_num |-> hdr_block *
+             log_start |=> log_blockset *
+             [[length log_blockset = log_length]] *
+             [[hdr = decode_header (fst hdr_block)]] *
+             [[log_blocks = map fst log_blockset]] *
+             [[old_count hdr <= cur_count hdr]] *
+             [[hash_valid (firstn (cur_count hdr) log_blocks) (cur_hash hdr)]] *
+             [[hash_valid (firstn (old_count hdr) log_blocks) (old_hash hdr)]] *
+             [[hashes_in_hashmap (snd a) hash0
+                                 (firstn (cur_count hdr) log_blocks)]] *
+             [[count_accurate hdr (length (txn_records hdr)) (cur_count hdr)]] *
+   [[count_accurate hdr (old_txn_count hdr) (old_count hdr)]] *
+   [[txns_valid hdr log_blocks (fst (fst a)) (snd (fst a))]] *
+          [[start >= log_start + cur_count hdr]] *
+          [[start + length vl < log_start + log_length]]));
+    unfold log_rep_inner; simpl; crush_pimpl.
+  
+  repeat (apply extract_exists; intros).
+  eapply post_impl.
+  eapply crash_impl.
+  eapply pre_impl.
+  eapply add_frame.
+  apply write_consecutive_ok.
+  {
+    crush_pimpl.
+    eassign (log_start |=> (firstn (start - log_start) v) *
+             hdr_block_num |-> v0 *
+             (start + length vl) |=> (skipn (length vl + (start - log_start)) v)).
+    cancel.
+    rewrite <- skipn_skipn.
+    eapply pimpl_trans. 
+    apply pred_array_split with (n:= start - log_start).
+    cancel.
+    rewrite Minus.le_plus_minus_r.
+    eapply pimpl_trans. 
+    apply pred_array_split with (n:= length vl).
+    cancel.
+    omega.
+    apply firstn_length_l.
+    rewrite skipn_length.
+    omega.
+  }
+  {
+    crush_pimpl.
+    eassign n.
+    eassign
+      (firstn (start - log_start) v ++
+       map_pointwise (map vsupd (firstn n vl))
+       (firstn n (firstn (length vl) (skipn (start - log_start) v))) ++
+        skipn (n + (start - log_start)) v).
+    unfold log_rep_inner.
+    repeat rewrite min_l; eauto.
+    cancel.
+    
+    eapply pimpl_trans. 
+    2: apply pred_array_merge with (n:= start - log_start).
+    rewrite skipn_app_eq; [| rewrite firstn_length_l; omega].
+    rewrite Minus.le_plus_minus_r; [| omega].
+    rewrite firstn_app2; [| rewrite firstn_length_l; omega].
+    cancel.
+
+    eapply pimpl_trans. 
+    2: apply pred_array_merge with (n:= n).
+    setoid_rewrite firstn_app2.
+    cancel.
+    rewrite skipn_app_eq.
+    rewrite le_plus_minus with (m:= length vl)(n:= n) at 3; eauto.
+    rewrite skipn_firstn_comm.
+    rewrite skipn_skipn.
+
+    eapply pimpl_trans. 
+    2: apply pred_array_merge with (n:= length vl - n).
+    cancel.
+    rewrite <- add_assoc.
+    rewrite Minus.le_plus_minus_r; eauto.
+    rewrite skipn_skipn.
+    rewrite add_assoc.
+    rewrite sub_add; eauto.
+
+    XXX.
+  
 Theorem read_header_ok :
   forall hdr o d a,
     << o, d, a >>
@@ -73,25 +239,32 @@ Theorem read_header_ok :
         [[ ar = a ]])%pred
       (log_rep hdr ar *
        [[ ar = a ]])%pred.
-Proof. Admitted. (*
+Proof. 
   unfold read_header; intros.
-  unfold log_rep, log_inner_rep.
+  eapply pre_impl.
+  2: eassign (fun (_: oracle) a => exists* hdr_block,
+      ((hdr_block_num |-> hdr_block *
+        (hdr_block_num |-> hdr_block --* log_rep hdr a)) *
+       [[ decode_header (fst hdr_block) = hdr ]]));
+  intros; apply log_rep_extract_header_block.
   repeat (apply extract_exists; intros).
   step.
-  { eassign (fun a => log_rep hdr a).
-    unfold log_rep, log_inner_rep; crush_pimpl.
-    cleanup; cancel.
+  { eassign (fun (_: oracle) a => log_rep hdr a).
+    crush_pimpl.
+    apply septract_ptsto_merge.
   }
 
-  { crush_pimpl.
-    cleanup; cancel. }
+  {
+    crush_pimpl.
+    apply septract_ptsto_merge.
+  }
 
   step.
-  { unfold log_rep, log_inner_rep; crush_pimpl. }
-  { unfold log_rep, log_inner_rep; crush_pimpl. }
 Qed.
-*)
+
 Hint Extern 1 (hoare_triple _ read_header _ _ _ _ _ _ _) => eapply read_header_ok : specs.
+
+
 
 Theorem commit_ok :
   forall hdr addr_l data_l o d a,
@@ -153,12 +326,15 @@ Proof.
       (* doable *)
       admit. }
 
+    intros.
     unfold log_rep.
     intros.
     apply extract_exists; intros.
+
     step.
     eapply write_consecutive_ok.
     (* need a septract type lemma here *)
+Abort.
 
 Theorem apply_txn_ok :
   forall txn log_blocks hdr txn_plain_blocks (disk_data: list data) o d a,
@@ -174,7 +350,7 @@ Theorem apply_txn_ok :
     let plain_data_blocks := skipn addr_count txn_plain_blocks in
     let addr_list := firstn data_count (blocks_to_addr_list plain_addr_blocks) in
     << o, d, a >>
-      (log_inner_rep log_blocks hdr kl em hm *
+      (log_inner_rep log_blocks hdr a *
        addr_list |L> disk_data *
        [[ length disk_data = data_count ]] *
        [[ In txn (txn_records hdr) ]] *
@@ -182,92 +358,72 @@ Theorem apply_txn_ok :
        [[ encryptionmap_valid em ]])
       (apply_txn txn log_blocks)
       << r, ar >>
-      (log_inner_rep log_blocks hdr kl em hm *
+      (log_inner_rep log_blocks hdr ar *
        addr_list |L> (map_pointwise (map vsupd plain_data_blocks) disk_data) * 
        [[ ar = a ]])%pred
       (exists* vsl',
-          log_inner_rep log_blocks hdr kl em hm *
+          log_inner_rep log_blocks hdr ar *
           addr_list |L> vsl' *
           [[ ar = a ]])%pred.
 Proof.
-  unfold apply_txn; intros.
-  destruct a, p; simpl fst; simpl snd.
-
-  eapply bind_ok.
+  unfold apply_txn; step.
   {
-    intros.
-    eapply pre_impl.
-    eapply add_frame.
-    apply decrypt_all_ok.
-    simpl.
-    eassign (log_inner_rep log_blocks hdr l e h * firstn (data_count txn) (blocks_to_addr_list (firstn (addr_count txn) txn_plain_blocks)) |L> disk_data).
     unfold log_inner_rep.
-    intros; cancel.
-    all: try eauto.
-    rewrite H4.
+    crush_pimpl.
 
+    rewrite H3.
     rewrite get_all_existing_encrypt_snd; eauto.
-    intros.
-    unfold cur_txns_valid in *.
-    specialize H9 with (1:= H5); cleanup.
-    rewrite H4 in *.
-    specialize H9 with (1:=H); cleanup; congruence.
+
+    intros; unfold cur_txns_valid in *.
+    specialize H8 with (1:= H4); cleanup.
+    rewrite H3 in *.
+    specialize H17 with (1:=H0); cleanup; congruence.
 
     unfold cur_txns_valid in *.
-    specialize H9 with (1:= H5); cleanup.
-    rewrite H4 in *.
+    specialize H8 with (1:= H4); cleanup.
+    rewrite H3 in *.
     rewrite map_length.
     symmetry; apply get_all_existing_encrypt_fst; eauto.
     intros.
     unfold cur_txns_valid in *.
-    specialize H7 with (1:= H9); cleanup; congruence.
+    specialize H8 with (1:= H17); cleanup; congruence.
   }
 
-  { intros; simpl; cancel.
-    instantiate (1:= fun ax => firstn (data_count txn) (blocks_to_addr_list (firstn (addr_count txn) txn_plain_blocks)) |L> disk_data * log_inner_rep log_blocks hdr (fst (fst ax)) (snd (fst ax)) (snd ax) ).
+  {
+    crush_pimpl.
+    instantiate (1:= fun _ ax => firstn (data_count txn) (blocks_to_addr_list (firstn (addr_count txn) txn_plain_blocks)) |L> disk_data * log_inner_rep log_blocks hdr ax).
     simpl; cancel. }
-  { intros; simpl; cancel. }
 
-  intros.
-  eapply bind_ok.
-  { intros.
-    eapply pre_impl.
-    eapply add_frame.
-    apply write_batch_ok.
+  step.
+  {
+    crush_pimpl.
+    rewrite get_all_existing_encrypt_snd; eauto.
 
-    {
-      simpl; intros; cancel.
-      repeat destruct_lifts; cleanup.
-      cancel.
-      destruct_lift H; cleanup.
-      rewrite get_all_existing_encrypt_snd; eauto.
-      cancel.
-      intros.
-      unfold log_inner_rep, cur_txns_valid in *.
-      destruct_lift H.
-      specialize H12 with (1:= H7); cleanup.
-      rewrite H6 in *.
-      specialize H10 with (1:=H1); cleanup; congruence.
-
-      destruct_lifts.
-      destruct_lift H; cleanup.
-      rewrite get_all_existing_encrypt_snd; eauto.
-
-      unfold log_inner_rep, cur_txns_valid in *.
-      destruct_lift H.
-      specialize H11 with (1:= H7); cleanup.
-      rewrite H6 in *.
-      simpl in *.    
-      rewrite skipn_length.
-      erewrite <- map_length, <- H6.
-      rewrite firstn_length_l.
-      rewrite Minus.minus_plus; eauto.
-      rewrite skipn_length.
-      rewrite H19.
-      unfold cur_count_accurate in *.
-      rewrite H13.
-      (* TODO: Figure out this goal *)
-      admit.
+    intros; unfold log_inner_rep, cur_txns_valid in *.
+    destruct_lifts.
+    specialize H22 with (1:= H7); cleanup.
+    rewrite H6 in *.
+    specialize H10 with (1:=H1); cleanup; congruence.
+    
+    destruct_lifts.
+    destruct_lift H; cleanup.
+    rewrite get_all_existing_encrypt_snd; eauto.
+    
+    unfold log_inner_rep, cur_txns_valid in *.
+    destruct_lift H.
+    specialize H11 with (1:= H7); cleanup.
+    rewrite H6 in *.
+    simpl in *.    
+    rewrite skipn_length.
+    erewrite <- map_length, <- H6.
+    rewrite firstn_length_l.
+    rewrite Minus.minus_plus; eauto.
+    rewrite skipn_length.
+    rewrite H19.
+    unfold cur_count_accurate in *.
+    rewrite H13.
+    (* TODO: Figure out this goal *)
+    admit.
       
       intros.
       unfold log_inner_rep, cur_txns_valid in *.
